examples/machine-code/acl2/m1_progScript.sml
@@ -20,11 +20,11 @@ val RW1 = ONCE_REWRITE_RULE;
 (* ----------------------------------------------------------------------------- *)
 
 val _ = Hol_datatype `
-  m1_el =   tPC     of sexp
-          | tLocals of sexp
-          | tStack  of sexp
-          | tInstr  of sexp => sexp
-          | tOK     of bool`;
+  m1_el =   tPC    of sexp
+          | tLocal of num => sexp
+          | tStack of sexp
+          | tInstr of sexp => sexp
+          | tOK    of bool`;
 
 val m1_el_11 = DB.fetch "-" "m1_el_11";
 val m1_el_distinct = DB.fetch "-" "m1_el_distinct";
@@ -37,12 +37,13 @@ val _ = Parse.type_abbrev("m1_set",``:m1_el set``);
 (* ----------------------------------------------------------------------------- *)
 
 val instr_def = Define `instr a s = nth a (program s)`;
+val nth_local_def = Define `nth_local a s = nth (nat a) (locals s)`;
 val m1_ok_def = Define `m1_ok s = ?x1 x2 x3 x4. s = make_state x1 x2 x3 x4`;
 
 val m1_2set'_def = Define `
-  m1_2set' (ps:unit set, ls: unit set, ss: unit set, is: sexp set, os: unit set) (s:sexp) =
+  m1_2set' (ps:unit set, ls: num set, ss: unit set, is: sexp set, os: unit set) (s:sexp) =
     IMAGE (\a. tPC (pc s)) ps UNION
-    IMAGE (\a. tLocals (locals s)) ls UNION
+    IMAGE (\a. tLocal a (nth_local a s)) ls UNION
     IMAGE (\a. tStack (stack s)) ss UNION
     IMAGE (\a. tInstr a (instr a s)) is UNION
     IMAGE (\a. tOK (m1_ok s)) os`;
@@ -72,7 +73,7 @@ val SUBSET_m1_2set = prove(
   \\ ASM_REWRITE_TAC [m1_2set'_SUBSET_m1_2set]
   \\ Q.EXISTS_TAC `(
        { a |a| ?x. tPC x IN u },
-       { a |a| ?x. tLocals x IN u },
+       { a |a| ?x. tLocal a x IN u },
        { a |a| ?x. tStack x IN u },
        { a |a| ?x. tInstr a x IN u },
        { a |a| ?x. tOK x IN u })`
@@ -91,13 +92,15 @@ val SPLIT_m1_2set_EXISTS = prove(
   \\ FULL_SIMP_TAC std_ss [EXTENSION,IN_DIFF,IN_UNION,DISJOINT_DEF,NOT_IN_EMPTY,IN_INTER]
   \\ METIS_TAC []);
 
+
+
 val IN_m1_2set = (SIMP_RULE std_ss [oneTheory.one] o prove)(``
   (!a x s. tPC x IN (m1_2set s) = (x = pc s)) /\
   (!a x s. tPC x IN (m1_2set' (ps,ls,ss,is,os) s) = (x = pc s) /\ a IN ps) /\
   (!a x s. tPC x IN (m1_2set'' (ps,ls,ss,is,os) s) = (x = pc s) /\ ~(a IN ps)) /\ 
-  (!a x s. tLocals x IN (m1_2set s) = (x = locals s)) /\
-  (!a x s. tLocals x IN (m1_2set' (ps,ls,ss,is,os) s) = (x = locals s) /\ a IN ls) /\
-  (!a x s. tLocals x IN (m1_2set'' (ps,ls,ss,is,os) s) = (x = locals s) /\ ~(a IN ls)) /\ 
+  (!a x s. tLocal a x IN (m1_2set s) = (x = nth_local a s)) /\
+  (!a x s. tLocal a x IN (m1_2set' (ps,ls,ss,is,os) s) = (x = nth_local a s) /\ a IN ls) /\
+  (!a x s. tLocal a x IN (m1_2set'' (ps,ls,ss,is,os) s) = (x = nth_local a s) /\ ~(a IN ls)) /\ 
   (!a x s. tStack x IN (m1_2set s) = (x = stack s)) /\
   (!a x s. tStack x IN (m1_2set' (ps,ls,ss,is,os) s) = (x = stack s) /\ a IN ss) /\
   (!a x s. tStack x IN (m1_2set'' (ps,ls,ss,is,os) s) = (x = stack s) /\ ~(a IN ss)) /\ 
@@ -124,8 +127,8 @@ val m1_2set''_11 = prove(
   THEN1 (`~((?y. tPC y IN m1_2set'' (ps,ls,ss,is,os) s) = 
             (?y. tPC y IN m1_2set'' (ps2,ls2,ss2,is2,os2) s'))` by 
          FULL_SIMP_TAC std_ss [IN_m1_2set,oneTheory.one] THEN1 METIS_TAC [])
-  THEN1 (`~((?y. tLocals y IN m1_2set'' (ps,ls,ss,is,os) s) = 
-            (?y. tLocals y IN m1_2set'' (ps2,ls2,ss2,is2,os2) s'))` by 
+  THEN1 (`~((?y. tLocal x y IN m1_2set'' (ps,ls,ss,is,os) s) = 
+            (?y. tLocal x y IN m1_2set'' (ps2,ls2,ss2,is2,os2) s'))` by 
          FULL_SIMP_TAC std_ss [IN_m1_2set,oneTheory.one] THEN1 METIS_TAC [])
   THEN1 (`~((?y. tStack y IN m1_2set'' (ps,ls,ss,is,os) s) = 
             (?y. tStack y IN m1_2set'' (ps2,ls2,ss2,is2,os2) s'))` by
@@ -140,7 +143,7 @@ val m1_2set''_11 = prove(
 val DELETE_m1_2set = (SIMP_RULE std_ss [oneTheory.one] o prove)(``
   (!a s. (m1_2set' (ps,ls,ss,is,os) s) DELETE tPC (pc s) =
          (m1_2set' (ps DELETE a,ls,ss,is,os) s)) /\ 
-  (!a s. (m1_2set' (ps,ls,ss,is,os) s) DELETE tLocals (locals s) =
+  (!a s. (m1_2set' (ps,ls,ss,is,os) s) DELETE tLocal a (nth_local a s) =
          (m1_2set' (ps,ls DELETE a,ss,is,os) s)) /\ 
   (!a s. (m1_2set' (ps,ls,ss,is,os) s) DELETE tStack (stack s) =
          (m1_2set' (ps,ls,ss DELETE a,is,os) s)) /\ 
@@ -165,7 +168,7 @@ val EMPTY_m1_2set = prove(``
 
 val tP_def = Define `tP x = SEP_EQ {tPC x}`;
 val tS_def = Define `tS x = SEP_EQ {tStack x}`;
-val tL_def = Define `tL x = SEP_EQ {tLocals x}`;
+val tL_def = Define `tL a x = SEP_EQ {tLocal a x}`;
 val tO_def = Define `tO x = SEP_EQ {tOK x}`;
 val tI_def = Define `tI a x = SEP_EQ {tInstr a x}`;
 
@@ -215,7 +218,7 @@ val EXPAND_STAR =
 
 val STAR_m1_2set = LIST_CONJ (map EXPAND_STAR 
   [``(tP x * p) (m1_2set' (ps,ls,ss,is,os) s)``,
-   ``(tL x * p) (m1_2set' (ps,ls,ss,is,os) s)``,
+   ``(tL a x * p) (m1_2set' (ps,ls,ss,is,os) s)``,
    ``(tS x * p) (m1_2set' (ps,ls,ss,is,os) s)``,
    ``(tI a x * p) (m1_2set' (ps,ls,ss,is,os) s)``,
    ``(tO x * p) (m1_2set' (ps,ls,ss,is,os) s)``]);
@@ -262,7 +265,7 @@ val IMP_M1_SPEC =
 val m1_2set''_thm = prove(
   ``(m1_2set'' (ps,ls,ss,is,os) s1 = m1_2set'' (ps,ls,ss,is,os) s2) =
     (!a. ~(a IN ps) ==> (pc s1 = pc s2)) /\
-    (!a. ~(a IN ls) ==> (locals s1 = locals s2)) /\
+    (!a. ~(a IN ls) ==> (nth_local a s1 = nth_local a s2)) /\
     (!a. ~(a IN ss) ==> (stack s1 = stack s2)) /\
     (!a. ~(a IN is) ==> (instr a s1 = instr a s2)) /\
     (!a. ~(a IN os) ==> (m1_ok s1 = m1_ok s2))``,
@@ -272,7 +275,7 @@ val m1_2set''_thm = prove(
   THEN1 (Cases \\ ASM_SIMP_TAC std_ss [IN_m1_2set] \\ METIS_TAC [])
   THEN1 (Q.PAT_ASSUM `!x.bb` (ASSUME_TAC o Q.SPEC `tPC (pc s1)`)
          \\ METIS_TAC [IN_m1_2set])
-  THEN1 (Q.PAT_ASSUM `!x.bb` (ASSUME_TAC o Q.SPEC `tLocals (locals s1)`)
+  THEN1 (Q.PAT_ASSUM `!x.bb` (ASSUME_TAC o Q.SPEC `tLocal a (nth_local a s1)`)
          \\ METIS_TAC [IN_m1_2set])
   THEN1 (Q.PAT_ASSUM `!x.bb` (ASSUME_TAC o Q.SPEC `tStack (stack s1)`)
          \\ METIS_TAC [IN_m1_2set])
@@ -505,10 +508,10 @@ val m1_ok_step = prove(
   \\ SIMP_TAC std_ss [m1_ok_def] \\ METIS_TAC []);  
 
 val IMP_SPEC_M1_MODEL = prove(
-  ``(!cs. (nth p1 cs = c) ==>
-          (step (make_state p1 l1 s1 cs) = make_state p2 l2 s2 cs)) ==>
-    SPEC M1_MODEL (tS s1 * tL l1 * PC p1)
-         {(p1,c)} (tS s2 * tL l2 * PC p2)``,
+  ``(!cs l1. (nth p1 cs = c) ==>
+             (step (make_state p1 l1 s1 cs) = make_state p2 l1 s2 cs)) ==>
+    SPEC M1_MODEL (tS s1 * PC p1)
+         {(p1,c)} (tS s2 * PC p2)``,
   REPEAT STRIP_TAC  
   \\ MATCH_MP_TAC IMP_M1_SPEC \\ SIMP_TAC std_ss [M1_NEXT_def]
   \\ SIMP_TAC std_ss [PC_def,GSYM STAR_ASSOC]
@@ -518,15 +521,60 @@ val IMP_SPEC_M1_MODEL = prove(
   \\ FULL_SIMP_TAC std_ss [m1_ok_def,make_state_thm,instr_def]
   \\ STRIP_TAC \\ RES_TAC \\ POP_ASSUM MP_TAC
   \\ Q.PAT_ASSUM `!cs.bb` (K ALL_TAC)
-  \\ ASM_SIMP_TAC std_ss [make_state_thm]);
+  \\ ASM_SIMP_TAC std_ss [make_state_thm,nth_local_def]);
+
+val IMP_SPEC_M1_MODEL_2 = prove(
+  ``(!cs l1. (nth p1 cs = c) /\ (v = nth (nat n) l1)  ==>
+             (step (make_state p1 l1 s1 cs) = make_state p2 l1 s2 cs)) ==>
+    SPEC M1_MODEL (tS s1 * tL n v * PC p1)
+         {(p1,c)} (tS s2 * tL n v * PC p2)``,
+  REPEAT STRIP_TAC  
+  \\ MATCH_MP_TAC IMP_M1_SPEC \\ SIMP_TAC std_ss [M1_NEXT_def]
+  \\ SIMP_TAC std_ss [PC_def,GSYM STAR_ASSOC]
+  \\ SIMP_TAC std_ss [pairTheory.FORALL_PROD,STAR_m1_2set,CODE_POOL_m1_2set,
+       UNIT_IN_SET,m1_2set''_thm,IN_INSERT,NOT_IN_EMPTY,oneTheory.one,instr_step]
+  \\ STRIP_TAC \\ Cases_on `m1_ok s` \\ ASM_SIMP_TAC std_ss [m1_ok_step]
+  \\ FULL_SIMP_TAC std_ss [m1_ok_def,make_state_thm,instr_def,nth_local_def]
+  \\ STRIP_TAC \\ STRIP_TAC \\ RES_TAC \\ POP_ASSUM MP_TAC
+  \\ Q.PAT_ASSUM `!cs.bb` (K ALL_TAC)
+  \\ ASM_SIMP_TAC std_ss [make_state_thm,nth_local_def]);
+
+val nth_update_nth = prove(
+  ``!n w l. (nth (nat n) (update_nth (nat n) w l) = w)``,
+  Induct \\ ASM_SIMP_TAC std_ss [nth_lemma,update_nth_lemma,car_def,cdr_def]);
+
+val nth_update_nth_NEQ = prove(
+  ``!n a w l. ~(n = a) ==> (nth (nat n) (update_nth (nat a) w l) = nth (nat n) l)``,
+  Induct \\ ASM_SIMP_TAC std_ss [nth_lemma,update_nth_lemma,car_def,cdr_def]
+  \\ Cases_on `a` \\ ASM_SIMP_TAC std_ss []
+  \\ ASM_SIMP_TAC std_ss [nth_lemma,update_nth_lemma,car_def,cdr_def]);
+
+val IMP_SPEC_M1_MODEL_3 = prove(
+  ``(!cs l1. (nth p1 cs = c) /\ (v = nth (nat n) l1)  ==>
+             (step (make_state p1 l1 s1 cs) = 
+              make_state p2 (update_nth (nat n) w l1) s2 cs)) ==>
+    SPEC M1_MODEL (tS s1 * tL n v * PC p1)
+         {(p1,c)} (tS s2 * tL n w * PC p2)``,
+  REPEAT STRIP_TAC  
+  \\ MATCH_MP_TAC IMP_M1_SPEC \\ SIMP_TAC std_ss [M1_NEXT_def]
+  \\ SIMP_TAC std_ss [PC_def,GSYM STAR_ASSOC]
+  \\ SIMP_TAC std_ss [pairTheory.FORALL_PROD,STAR_m1_2set,CODE_POOL_m1_2set,
+       UNIT_IN_SET,m1_2set''_thm,IN_INSERT,NOT_IN_EMPTY,oneTheory.one,instr_step]
+  \\ STRIP_TAC \\ Cases_on `m1_ok s` \\ ASM_SIMP_TAC std_ss [m1_ok_step]
+  \\ FULL_SIMP_TAC std_ss [m1_ok_def,make_state_thm,instr_def,nth_local_def]
+  \\ STRIP_TAC \\ STRIP_TAC \\ RES_TAC \\ POP_ASSUM MP_TAC
+  \\ Q.PAT_ASSUM `!cs.bb` (K ALL_TAC)
+  \\ ASM_SIMP_TAC std_ss [make_state_thm,nth_local_def,nth_update_nth]
+  \\ REPEAT STRIP_TAC \\ Cases_on `a = n` 
+  \\ FULL_SIMP_TAC std_ss [nth_update_nth_NEQ]);
 
 val acl2_ss = std_ss ++ rewrites [hol_defaxiomsTheory.ACL2_SIMPS,
   make_state_thm,nth_thm,CONS_11,NOT_CONS_NIL,stringTheory.CHR_11]  
 
-val M1_TAC = 
+fun M1_TAC thm = 
   SIMP_TAC std_ss [SPEC_MOVE_COND,precond_def] \\ SIMP_TAC std_ss [ACL2_TRUE] 
   \\ REPEAT STRIP_TAC
-  \\ MATCH_MP_TAC IMP_SPEC_M1_MODEL \\ ONCE_REWRITE_TAC defs2
+  \\ MATCH_MP_TAC thm \\ ONCE_REWRITE_TAC defs2
   \\ ASM_SIMP_TAC std_ss [make_state_thm,next_inst_defun]
   \\ REPEAT STRIP_TAC \\ POP_ASSUM (K ALL_TAC) \\ REPEAT (POP_ASSUM MP_TAC)
   \\ ONCE_REWRITE_TAC defs2 \\ SIMP_TAC acl2_ss [op_code_defun,List_def]  
@@ -537,70 +585,68 @@ val M1_TAC =
   \\ METIS_TAC [add_COMM]
 
 
-
 val M1_ICONST = store_thm("M1_ICONST",
   ``SPEC M1_MODEL
-       (tS s * tL l * PC p)
+       (tS s * PC p)
        {(p, List [sym "M1" "ICONST"; x])}
-       (tS (push x s) * tL l * PC (add p (nat 1)))``,
-  M1_TAC);
-
-val M1_ILOAD = store_thm("M1_ILOAD",
-  ``SPEC M1_MODEL
-       (tS s * tL l * PC p)
-       {(p, List [sym "M1" "ILOAD"; x])}
-       (tS (push (nth x l) s) * tL l * PC (add p (nat 1)))``,
-  M1_TAC);
-
-val M1_ISTORE = store_thm("M1_ISTORE",
-  ``SPEC M1_MODEL
-       (tS s * tL l * PC p)
-       {(p, List [sym "M1" "ISTORE"; x])}
-       (tS (pop s) * tL (update_nth x (top s) l) * PC (add p (nat 1)))``,
-  M1_TAC);
+       (tS (push x s) * PC (add p (nat 1)))``,
+  M1_TAC IMP_SPEC_M1_MODEL);
 
 val M1_IADD = store_thm("M1_IADD",
   ``SPEC M1_MODEL
-       (tS s * tL l * PC p)
+       (tS s * PC p)
        {(p, List [sym "M1" "IADD"])}
-       (tS (push (add (top (pop s)) (top s)) (pop (pop s))) * tL l * PC (add p (nat 1)))``,
-  M1_TAC);
+       (tS (push (add (top (pop s)) (top s)) (pop (pop s))) * PC (add p (nat 1)))``,
+  M1_TAC IMP_SPEC_M1_MODEL);
 
 val M1_ISUB = store_thm("M1_ISUB",
   ``SPEC M1_MODEL
-       (tS s * tL l * PC p)
+       (tS s * PC p)
        {(p, List [sym "M1" "ISUB"])}
-       (tS (push (add (top (pop s)) (unary_minus (top s))) (pop (pop s))) * tL l * PC (add p (nat 1)))``,
-  M1_TAC);
+       (tS (push (add (top (pop s)) (unary_minus (top s))) (pop (pop s))) * PC (add p (nat 1)))``,
+  M1_TAC IMP_SPEC_M1_MODEL);
 
 val M1_IMUL = store_thm("M1_IMUL",
   ``SPEC M1_MODEL
-       (tS s * tL l * PC p)
+       (tS s * PC p)
        {(p, List [sym "M1" "IMUL"])}
-       (tS (push (mult (top (pop s)) (top s)) (pop (pop s))) * tL l * PC (add p (nat 1)))``,
-  M1_TAC);
+       (tS (push (mult (top (pop s)) (top s)) (pop (pop s))) * PC (add p (nat 1)))``,
+  M1_TAC IMP_SPEC_M1_MODEL);
 
 val M1_GOTO = store_thm("M1_GOTO",
   ``SPEC M1_MODEL
-       (tS s * tL l * PC p)
+       (tS s * PC p)
        {(p, List [sym "M1" "GOTO"; x])}
-       (tS s * tL l * PC (add p x))``,
-  M1_TAC);
+       (tS s * PC (add p x))``,
+  M1_TAC IMP_SPEC_M1_MODEL);
 
 val M1_IFLE = store_thm("M1_IFLE",
   ``SPEC M1_MODEL
-       (tS s * tL l * PC p * precond ((|= (not (less (nat 0) (top s))))))
+       (tS s * PC p * precond ((|= (not (less (nat 0) (top s))))))
        {(p, List [sym "M1" "IFLE"; x])}
-       (tS (pop s) * tL l * PC (add p x))``,
-  M1_TAC);
+       (tS (pop s) * PC (add p x))``,
+  M1_TAC IMP_SPEC_M1_MODEL);
 
 val M1_IFLE_NOP = store_thm("M1_IFLE_NOP",
   ``SPEC M1_MODEL
-       (tS s * tL l * PC p * precond (~(|= (not (less (nat 0) (top s))))))
+       (tS s * PC p * precond (~(|= (not (less (nat 0) (top s))))))
        {(p, List [sym "M1" "IFLE"; x])}
-       (tS (pop s) * tL l * PC (add p (nat 1)))``,
-  M1_TAC);
+       (tS (pop s) * PC (add p (nat 1)))``,
+  M1_TAC IMP_SPEC_M1_MODEL);
 
+val M1_ILOAD = store_thm("M1_ILOAD",
+  ``SPEC M1_MODEL
+       (tS s * tL n v * PC p)
+       {(p, List [sym "M1" "ILOAD"; (nat n)])}
+       (tS (push v s) * tL n v * PC (add p (nat 1)))``,
+  M1_TAC IMP_SPEC_M1_MODEL_2);
+
+val M1_ISTORE = store_thm("M1_ISTORE",
+  ``SPEC M1_MODEL
+       (tS s * tL n v * PC p)
+       {(p, List [sym "M1" "ISTORE"; (nat n)])}
+       (tS (pop s) * tL n (top s) * PC (add p (nat 1)))``,
+  M1_TAC IMP_SPEC_M1_MODEL_3);
 
     
 val _ = export_theory();
